Mlir/Rewriter/Basic.lean
@@ -1,2 +1,579 @@
-import Mlir.Rewriter.Rewriter
-import Mlir.Rewriter.Builder
+import Mlir.Core
+import Mlir.Rewriter.LinkedList
+
+namespace Mlir
+
+/--
+- A position in the IR where we can insert an operation.
+-/
+inductive InsertPoint where
+  | Before (op: OperationPtr)
+  | AtEnd (block: BlockPtr)
+deriving DecidableEq
+
+@[grind]
+def InsertPoint.InBounds : InsertPoint → IRContext → Prop
+| Before op => op.InBounds
+| AtEnd bl => bl.InBounds
+
+@[grind =]
+theorem InsertPoint.inBounds_before : (Before op).InBounds ctx ↔ op.InBounds ctx := by rfl
+@[grind =]
+theorem InsertPoint.inBounds_atEnd : (AtEnd bl).InBounds ctx ↔ bl.InBounds ctx := by rfl
+
+@[grind]
+def InsertPoint.block! (insertionPoint : InsertPoint) (ctx : IRContext) : Option BlockPtr :=
+  match insertionPoint with
+  | InsertPoint.Before op => (op.get! ctx).parent
+  | InsertPoint.AtEnd b => b
+
+def InsertPoint.block (insertionPoint : InsertPoint) (ctx : IRContext)
+    (hIn : insertionPoint.InBounds ctx := by grind) : Option BlockPtr :=
+  match insertionPoint with
+  | InsertPoint.Before op => (op.get ctx (by grind)).parent
+  | InsertPoint.AtEnd b => b
+
+@[grind =]
+theorem InsertPoint.block!_eq_block (insertionPoint : InsertPoint) (ctx : IRContext)
+    (hIn : insertionPoint.InBounds ctx) :
+    insertionPoint.block! ctx = insertionPoint.block ctx hIn := by
+  cases insertionPoint <;> grind [InsertPoint.block!, InsertPoint.block]
+
+@[grind .]
+theorem InsertPoint.block_InBounds {insertionPoint : InsertPoint} {ctx : IRContext}
+    (ctxFieldsInBounds : ctx.FieldsInBounds) (hIn : insertionPoint.InBounds ctx) :
+    insertionPoint.block ctx hIn = some blockPtr →
+    insertionPoint.InBounds ctx →
+    blockPtr.InBounds ctx := by
+  simp only [InsertPoint.block]
+  grind
+
+/- set_option pp.proofs true -/
+/- set_option pp.showLetValues true -/
+
+/--
+- Insert an operation at a given location.
+-/
+@[grind]
+def Rewriter.insertOp? (ctx: IRContext) (newOp: OperationPtr) (insertionPoint: InsertPoint)
+    (newOpIn: newOp.InBounds ctx := by grind)
+    (insIn : insertionPoint.InBounds ctx)
+    (ctxInBounds: ctx.FieldsInBounds) : Option IRContext :=
+  match _ : insertionPoint with
+    | InsertPoint.Before existingOp =>
+      rlet parent ← (existingOp.get ctx (by grind)).parent
+      let prev := (existingOp.get ctx (by grind)).prev
+      let next := some existingOp
+      newOp.linkBetweenWithParent ctx prev next parent (by grind) (by grind) (by grind) (by grind)
+    | InsertPoint.AtEnd block =>
+      let parent := block
+      let prev := (block.get ctx (by grind)).lastOp
+      let next := none
+      newOp.linkBetweenWithParent ctx prev next parent (by grind) (by grind) (by grind) (by grind)
+
+@[irreducible]
+def Rewriter.detachOp (ctx: IRContext) (hctx : ctx.FieldsInBounds) (op: OperationPtr) (hIn : op.InBounds ctx) (hasParent: (op.get ctx hIn).parent.isSome) : IRContext :=
+  let opStruct := op.get ctx
+  let parent := opStruct.parent.get hasParent
+  let ctx := op.setParent ctx none
+  let prevOp := opStruct.prev
+  let nextOp := opStruct.next
+  -- Leo: I had to duplicate the continuation in each branch, I don't really
+  -- know why the proofs of the preconditions in, say, `setNextOp` were
+  -- metavariable... maybe somehow the execution of the tactics is slightly
+  -- delayed?
+  match _ : prevOp with
+    | some prevOp =>
+      let ctx := prevOp.setNextOp ctx nextOp
+      match _ : nextOp with
+      | some nextOp => nextOp.setPrevOp ctx prevOp (by grind (ematch := 10))
+      | none => parent.setLastOp ctx prevOp (by grind (ematch := 10))
+    | none =>
+      let ctx := parent.setFirstOp ctx nextOp
+      match _ : nextOp with
+      | some nextOp => nextOp.setPrevOp ctx prevOp (by grind (ematch := 10))
+      | none => parent.setLastOp ctx prevOp
+
+@[grind .]
+theorem Rewriter.detachOp_inBounds (ptr : GenericPtr) :
+    ptr.InBounds (detachOp ctx hctx op hIn hasParent) ↔ ptr.InBounds ctx := by
+  grind [detachOp]
+
+@[grind .]
+theorem Rewriter.detachOp_fieldsInBounds (hctx : ctx.FieldsInBounds) :
+    (detachOp ctx hctx op hIn hasParent).FieldsInBounds := by
+  simp only [detachOp]
+  split <;> grind
+
+/--
+- Erase an operation and free it from memory.
+- TODO: free memory here
+-/
+
+@[irreducible, inline]
+def Rewriter.eraseOpStart (ctx: IRContext) (hctx : ctx.FieldsInBounds) (op: OperationPtr) (hop : op.InBounds ctx) (hasParent: (op.get ctx hop).parent.isSome) := Id.run do
+  let mut newCtx : { c : IRContext // c.FieldsInBounds ∧ ∀ (ptr : GenericPtr), ptr.InBounds ctx ↔ ptr.InBounds c} :=
+    ⟨Rewriter.detachOp ctx hctx op hop hasParent, by grind⟩
+  for h : index in 0 ... (op.getNumOperands ctx (by grind)) do
+    let ctx' := (OpOperandPtr.mk op index).removeFromCurrent newCtx (by
+       have := newCtx.property.2 (.opOperand (.mk op index))
+       grind [OperationPtr.getNumOperands, OpOperandPtr.InBounds]) (by grind) -- TODO: try to not unfold `get`, maybe some lemma for op.InBounds + index < .. → (.mk op index).InBounds
+    newCtx := ⟨ctx', by grind⟩
+  newCtx
+
+@[grind .]
+theorem Rewriter.eraseOpStart_inBounds (ptr : GenericPtr) :
+    ptr.InBounds (eraseOpStart ctx hctx op hIn hasParent) ↔ ptr.InBounds ctx := by
+  grind
+
+@[grind .]
+theorem Rewriter.eraseOpStart_fieldsInBounds :
+    ctx.FieldsInBounds → (eraseOpStart ctx hctx op hIn hasParent).val.FieldsInBounds := by
+  grind
+
+@[irreducible]
+def Rewriter.eraseOp (ctx: IRContext) (op: OperationPtr) (hctx : ctx.FieldsInBounds := by grind)
+    (hop : op.InBounds ctx := by grind) (hasParent: (op.get ctx hop).parent.isSome := by grind) : IRContext := Id.run do
+  let ctx := eraseOpStart ctx hctx op hop hasParent
+  { ctx.val with operations := ctx.val.operations.erase op }
+
+/-
+Remark: the fact that `eraseOp` preserves `FieldsInBounds` relies on the fact
+that the context is well formed.  Indeed, it is true because the only pointers
+to the operands are in the doubly linked list that we patch.  I think in
+addition we need to know that the results of the operation we are removing are
+never used, which is ensured in the call to `eraseOp` in `replaceOp?` below for
+example.
+-/
+
+/--
+- A position in the IR where we can insert an operation.
+-/
+inductive BlockInsertPoint where
+  | Before (op: BlockPtr)
+  | AtEnd (block: RegionPtr)
+
+@[grind]
+def BlockInsertPoint.InBounds : BlockInsertPoint → IRContext → Prop
+| Before op => op.InBounds
+| AtEnd bl => bl.InBounds
+@[grind =]
+theorem BlockInsertPoint.inBounds_before : (Before op).InBounds ctx ↔ op.InBounds ctx := by rfl
+@[grind =]
+theorem BlockInsertPoint.inBounds_atEnd : (AtEnd bl).InBounds ctx ↔ bl.InBounds ctx := by rfl
+
+@[irreducible]
+private def Rewriter.insertBlockAfter? (ctx: IRContext) (newBlock: BlockPtr) (existingBlock: BlockPtr)
+    (newBlockIn: newBlock.InBounds ctx := by grind)
+    (existingBlockIn: existingBlock.InBounds ctx := by grind)
+    (ctxInBounds: ctx.FieldsInBounds) : Option IRContext := do
+  rlet parent ← (existingBlock.get ctx (by grind)).parent
+  let ctx := existingBlock.linkNextBlock ctx newBlock
+  rlet ctx ← newBlock.setParentWithCheck ctx parent (by grind)
+  let nextBlock := (newBlock.get ctx (by grind)).next
+  if h : nextBlock = none then
+    parent.setLastBlock ctx (some newBlock) (by grind (ematch := 10))
+  else
+    ctx
+
+@[irreducible]
+private def Rewriter.insertBlockBefore? (ctx: IRContext) (newBlock: BlockPtr) (existingBlock: BlockPtr)
+    (newBlockIn: newBlock.InBounds ctx := by grind)
+    (existingBlockIn: existingBlock.InBounds ctx := by grind)
+    (ctxInBounds: ctx.FieldsInBounds) : Option IRContext := do
+  rlet parent ← (existingBlock.get ctx (by grind)).parent
+  let ctx := existingBlock.linkPrevBlock ctx newBlock
+  rlet ctx ← newBlock.setParentWithCheck ctx parent (by grind)
+  let prevBlock := (newBlock.get ctx (by grind)).prev
+  if h : prevBlock = none then
+    return parent.setFirstBlock ctx (some newBlock) (by grind (ematch := 10))
+  else
+    ctx
+
+@[irreducible]
+private def Rewriter.insertBlockInEmptyRegion? (ctx: IRContext) (newBlock: BlockPtr) (region: RegionPtr)
+    (newBlockIn: newBlock.InBounds ctx := by grind)
+    (regionIn: region.InBounds ctx := by grind) : Option IRContext := do
+  rlet ctx ← newBlock.setParentWithCheck ctx region (by grind)
+  let ctx := region.setFirstBlock ctx (some newBlock)
+  let ctx := region.setLastBlock ctx (some newBlock)
+  let ctx := newBlock.setPrevBlock ctx none
+  let ctx := newBlock.setNextBlock ctx none
+  return ctx
+
+/--
+- Insert a block at a given location.
+-/
+@[irreducible]
+def Rewriter.insertBlock? (ctx: IRContext) (newBlock: BlockPtr) (insertionPoint:
+    BlockInsertPoint) (hib : insertionPoint.InBounds ctx := by grind)
+    (newBlockIn: newBlock.InBounds ctx := by grind)
+    (ctxInBounds: ctx.FieldsInBounds := by grind) : Option IRContext :=
+  match h : insertionPoint with
+  | BlockInsertPoint.Before existingBlock =>
+    Rewriter.insertBlockBefore? ctx newBlock existingBlock (by grind) (by grind) ctxInBounds
+  | BlockInsertPoint.AtEnd region =>
+    match h : (region.get ctx (by grind)).lastBlock with
+    | none => Rewriter.insertBlockInEmptyRegion? ctx newBlock region (by grind) (by grind)
+    | some lastBlock => Rewriter.insertBlockAfter? ctx newBlock lastBlock (by grind) (by grind) ctxInBounds
+
+def Rewriter.replaceUse (ctx: IRContext) (use : OpOperandPtr) (newValue: ValuePtr)
+    (useIn: use.InBounds ctx := by grind)
+    (newIn: newValue.InBounds ctx := by grind)
+    (ctxIn: ctx.FieldsInBounds := by grind) : IRContext :=
+  if (use.get ctx (by grind)).value = newValue then
+    ctx
+  else
+    let ctx := use.removeFromCurrent ctx (by grind) (by grind)
+    let ctx := use.setValue ctx newValue
+    let ctx := use.insertIntoCurrent ctx (by grind) (by grind)
+    ctx
+
+@[grind =]
+theorem Rewriter.replaceUse_inBounds (ptr : GenericPtr) :
+    ptr.InBounds (replaceUse ctx use newValue useIn newIn ctxIn) ↔ ptr.InBounds ctx := by
+  grind [replaceUse]
+
+@[grind .]
+theorem Rewriter.replaceUse_fieldsInBounds :
+     ctx.FieldsInBounds → (replaceUse ctx use newValue useIn newIn ctxIn).FieldsInBounds := by
+  grind [replaceUse]
+
+@[irreducible]
+def Rewriter.replaceValue? (ctx: IRContext) (oldValue: ValuePtr) (newValue: ValuePtr)
+    (oldIn: oldValue.InBounds ctx := by grind)
+    (newIn: newValue.InBounds ctx := by grind)
+    (ctxIn: ctx.FieldsInBounds := by grind)
+    (depth: Nat := 1_000_000_000) : Option IRContext :=
+  match depth with
+  | Nat.succ depth =>
+    match _ : oldValue.getFirstUse ctx (by grind) with
+    | none => ctx
+    | some firstUse =>
+    let ctx := Rewriter.replaceUse ctx firstUse newValue
+    Rewriter.replaceValue? ctx oldValue newValue (by grind [Rewriter.replaceUse]) (by grind [Rewriter.replaceUse]) (by grind [Rewriter.replaceUse]) depth
+  | _ => none
+
+@[grind .]
+theorem Rewriter.replaceValue?_inBounds (ptr : GenericPtr) :
+    replaceValue? ctx old new h₁ h₂ h₃ d = some ctx' →
+    (ptr.InBounds ctx ↔ ptr.InBounds ctx') := by
+  induction d generalizing ctx
+  case zero => simp [replaceValue?]
+  case succ d ih => simp [replaceValue?]; split <;> grind [Rewriter.replaceUse]
+
+@[grind .]
+theorem Rewriter.replaceValue?_fieldsInBounds :
+     ctx.FieldsInBounds → (replaceValue? ctx old new h₁ h₂ h₃ d).maybe₁ IRContext.FieldsInBounds := by
+  induction d generalizing ctx
+  case zero => simp [replaceValue?, Option.maybe₁]
+  case succ d ih => simp [replaceValue?]; grind [Rewriter.replaceUse]
+
+@[grind .]
+theorem Rewriter.replaceValue?_preserves_results_size' (op : OperationPtr) (hop : op.InBounds ctx) :
+    replaceValue? ctx old new h₁ h₂ h₃ d = some ctx' →
+    op.getNumResults! ctx' = op.getNumResults! ctx := by
+  induction d generalizing ctx ctx'
+  case zero => simp [replaceValue?, *]
+  case succ d ih =>
+    simp only [replaceValue?]; split
+    · grind
+    · rename_i firstUse hFirstUse
+      intros hh
+      rw [ih (ctx' := ctx') (ctx := Rewriter.replaceUse ctx firstUse new (by grind) (by grind) (by grind))] <;> grind [Rewriter.replaceUse]
+
+@[grind .]
+theorem Rewriter.replaceValue?_preserves_results_size (op : OperationPtr) (hop : op.InBounds ctx)
+    (hctx' : replaceValue? ctx old new h₁ h₂ h₃ d = some ctx') :
+    op.getNumResults! ctx' = op.getNumResults! ctx  := by
+  have := @replaceValue?_preserves_results_size'
+  grind
+
+@[grind .]
+theorem Rewriter.replaceValue?_preserves_parent' (op : OperationPtr) (hop : op.InBounds ctx)
+    (hctx' : replaceValue? ctx old new h₁ h₂ h₃ d = some ctx') :
+    (op.get! ctx').parent = (op.get! ctx).parent := by
+  induction d generalizing ctx
+  case zero => simp [replaceValue?, *] at hctx' ⊢
+  case succ d ih =>
+    simp only [replaceValue?] at hctx'; split at hctx'
+    · grind
+    · rename_i firstUse hFirstUse
+      rw [ih (ctx := Rewriter.replaceUse ctx firstUse new (by grind) (by grind) (by grind)) (by grind [Rewriter.replaceUse])] <;> grind [Rewriter.replaceUse]
+
+@[grind .]
+theorem Rewriter.replaceValue?_preserves_parent (op : OperationPtr) (hop : op.InBounds ctx)
+    (hctx' : replaceValue? ctx old new h₁ h₂ h₃ d = some ctx') :
+    (op.get ctx' (by grind)).parent = (op.get ctx hop).parent := by
+  have := @replaceValue?_preserves_parent'
+  grind [Rewriter.replaceUse]
+
+@[irreducible]
+def Rewriter.replaceValues (ctx: IRContext) (values: List (ValuePtr × ValuePtr)) : Option IRContext :=
+  values.foldlM (init := ctx) fun ctx (oldValue, newValue) =>
+    Rewriter.replaceValue? ctx oldValue newValue (by sorry) (by sorry) (by sorry)
+
+@[irreducible]
+def Rewriter.replaceOp? (ctx: IRContext) (oldOp newOp: OperationPtr)
+    (oldIn: oldOp.InBounds ctx := by grind)
+    (newIn: newOp.InBounds ctx := by grind)
+    (ctxIn: ctx.FieldsInBounds := by grind)
+    (hpar : (oldOp.get ctx).parent.isSome = true) : Option IRContext := do
+  let numOldResults := oldOp.getNumResults ctx (by grind)
+  let numNewResults := newOp.getNumResults ctx (by grind)
+  if h : numOldResults ≠ numNewResults then
+    none
+  else
+    let mut newCtx : { c: IRContext //
+        c.FieldsInBounds ∧
+        (∀ (ptr : GenericPtr), ptr.InBounds c ↔ ptr.InBounds ctx) ∧
+        (∀ (op : OperationPtr), ∀ h₁ h₂, (op.getNumResults ctx h₁) = (op.getNumResults c h₂)) ∧
+        (∀ (op : OperationPtr), ∀ h₁ h₂, (op.get ctx h₁).parent = (op.get c h₂).parent) } :=
+      ⟨ctx, by grind⟩
+    for h : i in 0...numOldResults do
+      let oldResult := oldOp.getResult i
+      let newResult := newOp.getResult i
+      -- TODO: fix and use rlet
+      match _ : (Rewriter.replaceValue? newCtx oldResult newResult (by grind) (by grind) (by grind)) with
+      | none => none
+      | some newCtxNoProof =>
+        newCtx := ⟨newCtxNoProof, (by grind)⟩
+    return Rewriter.eraseOp newCtx oldOp
+
+
+@[irreducible]
+def Rewriter.createBlock (ctx: IRContext) (insertionPoint: Option BlockInsertPoint)
+    (hctx : ctx.FieldsInBounds) (hip : insertionPoint.maybe BlockInsertPoint.InBounds ctx)
+    : Option (IRContext × BlockPtr) :=
+  rlet (ctx, newBlockPtr) ← BlockPtr.allocEmpty ctx
+  match h : insertionPoint with
+  | some insertionPoint => do
+    let ctx ← Rewriter.insertBlock? ctx newBlockPtr insertionPoint (by grind [Option.maybe, cases BlockInsertPoint])
+    (ctx, newBlockPtr)
+  | none =>
+    (ctx, newBlockPtr)
+
+@[irreducible, grind]
+def Rewriter.createRegion (ctx: IRContext) : Option (IRContext × RegionPtr) :=
+  RegionPtr.allocEmpty ctx
+
+@[irreducible]
+def Rewriter.initOpRegions (ctx: IRContext) (opPtr: OperationPtr) (numRegions: Nat)
+    (hop : opPtr.InBounds ctx) : Option IRContext :=
+  match numRegions with
+  | 0 => some ctx
+  | Nat.succ n => do
+    rlet (ctx, regionPtr) ← Rewriter.createRegion ctx
+    let oldRegion := regionPtr.get ctx (by grind)
+    let ctx := opPtr.setRegions ctx ((opPtr.get ctx).regions.push regionPtr)
+    Rewriter.initOpRegions ctx opPtr n (by grind)
+
+@[grind .]
+theorem Rewriter.initOpRegions_fieldsInBounds
+    (hx : ctx.FieldsInBounds)
+    (heq : initOpRegions ctx opPtr numRegions h₁ = some ctx') :
+    ctx'.FieldsInBounds := by
+  induction numRegions generalizing ctx <;> sorry --grind [initOpRegions]
+
+@[grind .]
+theorem Rewriter.initOpRegions_inBounds_mono (ptr : GenericPtr)
+    (heq : initOpRegions ctx opPtr numRegions h₁ = some ctx') :
+    ptr.InBounds ctx → ptr.InBounds ctx' := by
+  induction numRegions generalizing ctx <;>
+    grind [initOpRegions, Option.unattach_eq_some_iff]
+
+@[irreducible]
+def Rewriter.initOpResults (ctx: IRContext) (opPtr: OperationPtr) (numResults: Nat) (index: Nat := 0) (hop : opPtr.InBounds ctx)
+    (hidx : index = opPtr.getNumResults ctx) : IRContext :=
+  match numResults with
+  | 0 => ctx
+  | Nat.succ n =>
+    let result: OpResult := { type := (), firstUse := none, index := index, owner := opPtr }
+    let ctx := opPtr.pushResult ctx result
+    have : opPtr.InBounds ctx := by grind
+    have : result.FieldsInBounds ctx := by
+      -- TODO(later): write the right lemma somewhere.
+      constructor <;> grind [OperationPtr.pushResult, OperationPtr.setResults, OperationPtr.set, OperationPtr.get]
+    Rewriter.initOpResults ctx opPtr n (index + 1) (by grind) (by grind)
+
+@[grind .]
+theorem Rewriter.initOpResults_fieldsInBounds (hx : ctx.FieldsInBounds) :
+    (initOpResults ctx opPtr numResults index h₁ h₂).FieldsInBounds := by
+  induction numResults generalizing ctx index
+  · grind [initOpResults]
+  case succ numResults ih =>
+    simp [initOpResults]
+    apply ih
+    apply OperationPtr.pushResult_fieldsInBounds
+    · constructor <;> grind [OperationPtr.pushResult, OperationPtr.setResults, OperationPtr.set, OperationPtr.get]
+    · grind
+
+@[grind .]
+theorem Rewriter.initOpResults_inBounds_mono (ptr : GenericPtr) :
+    ptr.InBounds ctx → ptr.InBounds (initOpResults ctx opPtr numResults index h₁ h₂) := by
+  induction numResults generalizing ctx index <;> grind [initOpResults]
+
+@[irreducible]
+protected def Rewriter.pushOperand (ctx : IRContext) (opPtr : OperationPtr) (valuePtr : ValuePtr)
+    (opPtrInBounds : opPtr.InBounds ctx := by grind) (valueInBounds : valuePtr.InBounds ctx := by grind) (hctx : ctx.FieldsInBounds) : IRContext :=
+  let op := (opPtr.get ctx (by grind))
+  let index := opPtr.getNumOperands ctx (by grind)
+  let operand := { value := valuePtr, owner := opPtr, back := OpOperandPtrPtr.valueFirstUse valuePtr, nextUse := none : OpOperand}
+  have : operand.FieldsInBounds ctx := by constructor <;> grind [Option.maybe]
+  let ctx := opPtr.pushOperand ctx operand (by grind)
+  let ctx := (OpOperandPtr.mk opPtr index).insertIntoCurrent ctx (by grind) (by grind)
+  ctx
+
+@[grind .]
+theorem Rewriter.pushOperand_inBounds (ptr : GenericPtr) :
+    ptr.InBounds (Rewriter.pushOperand ctx opPtr valuePtr h₁ h₂ h₃) ↔
+    (ptr.InBounds ctx ∨
+     ptr = .opOperand ⟨opPtr, (opPtr.getNumOperands ctx)⟩ ∨
+     ptr = .opOperandPtr (.operandNextUse ⟨opPtr, (opPtr.getNumOperands ctx)⟩)) := by
+  grind [Rewriter.pushOperand]
+
+@[grind .]
+theorem Rewriter.pushOperand_inBounds_mono (ptr : GenericPtr) :
+    ptr.InBounds ctx → ptr.InBounds (Rewriter.pushOperand ctx opPtr valuePtr h₁ h₂ h₃) := by
+  grind
+
+@[grind .]
+theorem Rewriter.pushOperand_fieldsInBounds :
+    (Rewriter.pushOperand ctx opPtr valuePtr h₁ h₂ h₃).FieldsInBounds := by
+  grind [Rewriter.pushOperand]
+
+@[irreducible]
+def Rewriter.initOpOperands (ctx: IRContext) (opPtr: OperationPtr) (opPtrInBounds : opPtr.InBounds ctx)
+    (operands : Array ValuePtr) (hoperands : ∀ oper, oper ∈ operands → oper.InBounds ctx) (hctx : ctx.FieldsInBounds)
+    (n : Nat := operands.size) (hn : 0 ≤ n ∧ n ≤ operands.size := by grind) : IRContext :=
+  match h : n with
+  | 0 => ctx
+  | Nat.succ n' =>
+    let index := operands.size - n
+    let valuePtr := operands[index]'(by grind)
+    let ctx := Rewriter.pushOperand ctx opPtr valuePtr (by grind) (by grind) (by grind)
+    Rewriter.initOpOperands ctx opPtr (by grind) operands (by grind) (by grind) n' (by grind)
+
+@[grind .]
+theorem Rewriter.initOpOperands_fieldsInBounds :
+    (initOpOperands ctx opPtr h₁ operands h₂ h₃ n hn).FieldsInBounds := by
+  induction n generalizing ctx
+  case zero => grind [initOpOperands]
+  case succ n ih =>
+    simp [initOpOperands]
+    grind
+
+@[grind .]
+theorem Rewriter.initOpOperands_inBounds_mono (ptr : GenericPtr) :
+    ptr.InBounds ctx → ptr.InBounds (initOpOperands ctx opPtr h₁ operands h₂ h₃ n hn) := by
+  induction n generalizing ctx
+  case zero => grind [initOpOperands]
+  case succ n ih =>
+    simp [initOpOperands]
+    grind
+
+@[irreducible]
+private def Rewriter.createEmptyOp (ctx : IRContext) (opType : Nat) : Option (IRContext × OperationPtr) :=
+  OperationPtr.allocEmpty ctx opType
+
+@[grind .]
+theorem Rewriter.createEmptyOp_new_inBounds (h : createEmptyOp ctx opType = some (ctx', op)) :
+    op.InBounds ctx' := by
+  grind [createEmptyOp]
+
+@[grind .]
+theorem Rewriter.createEmptyOp_genericPtr_mono (ptr : GenericPtr) (heq : createEmptyOp ctx type = some (ctx', ptr')) :
+    ptr.InBounds ctx' ↔ (ptr.InBounds ctx ∨ ptr = .operation ptr') := by
+  grind [createEmptyOp, OperationPtr.allocEmpty_genericPtr_iff']
+
+@[grind .]
+theorem Rewriter.createEmptyOp_fieldsInBounds (h : createEmptyOp ctx opType = some (ctx', op)) :
+    ctx.FieldsInBounds → ctx'.FieldsInBounds := by
+  grind [createEmptyOp]
+
+
+@[irreducible]
+def Rewriter.createOp (ctx: IRContext) (opType: Nat)
+    (numResults: Nat) (operands: Array ValuePtr) (numRegions: Nat) (properties: UInt64)
+    (insertionPoint: Option InsertPoint)
+    (hoper : ∀ oper, oper ∈ operands → oper.InBounds ctx)
+    (hins : insertionPoint.maybe InsertPoint.InBounds ctx)
+    (hx : ctx.FieldsInBounds) : Option (IRContext × OperationPtr) :=
+  rlet (ctx, newOpPtr) ← Rewriter.createEmptyOp ctx opType
+  have hib : newOpPtr.InBounds ctx := by grind
+  have : (newOpPtr.get ctx (by grind)).results = #[] := by
+    grind [createEmptyOp, OperationPtr.allocEmpty, Operation.empty]
+  let ctx := Rewriter.initOpResults ctx  newOpPtr numResults 0 (by grind) (by grind [OperationPtr.getNumResults])
+  let ctx := newOpPtr.setProperties ctx properties
+  rlet ctx ← Rewriter.initOpRegions ctx newOpPtr numRegions (by grind)
+  let ctx := Rewriter.initOpOperands ctx newOpPtr (by grind) operands (by grind) (by grind)
+  match _ : insertionPoint with
+  | some insertionPoint =>
+    rlet ctx ← Rewriter.insertOp? ctx newOpPtr insertionPoint (by grind) (by cases insertionPoint <;> grind [Option.maybe]) (by grind) in
+    some (ctx, newOpPtr)
+  | none =>
+    (ctx, newOpPtr)
+
+abbrev ModuleTypeID := 0
+
+unseal Rewriter.createRegion in
+@[irreducible]
+def IRContext.create : Option (IRContext × OperationPtr) :=
+  let ctx : IRContext := {
+    nextID := 0,
+    operations := Std.HashMap.emptyWithCapacity,
+    blocks := Std.HashMap.emptyWithCapacity,
+    regions := Std.HashMap.emptyWithCapacity,
+    topLevelOp := 0
+  }
+  -- Note: We inline part of the definition of `createOp` because the above
+  -- `ctx` does not satisfy `ctx.FieldsInBounds` because `topLevelOp` is an
+  -- invalid pointer.
+  rlet (ctx, operation) ← Rewriter.createEmptyOp ctx ModuleTypeID
+  have hib : operation.InBounds ctx := by grind
+  have : ctx.topLevelOp = 0 := by
+    grind [Rewriter.createEmptyOp, OperationPtr.allocEmpty, Operation.empty, OperationPtr.set]
+  have hops : ∀ (op : OperationPtr), op.InBounds ctx ↔ op = 0 := by
+    grind [Rewriter.createEmptyOp, OperationPtr.allocEmpty, Operation.empty, OperationPtr.set, OperationPtr.InBounds]
+  have : (operation.get ctx (by grind)).results = #[] := by
+    grind [Rewriter.createEmptyOp, OperationPtr.allocEmpty, Operation.empty]
+  have : ∀ (bl : BlockPtr), bl.InBounds ctx ↔ False := by
+    grind [Rewriter.createEmptyOp, OperationPtr.allocEmpty, Operation.empty, OperationPtr.set, BlockPtr.InBounds]
+  have : ∀ (r : RegionPtr), r.InBounds ctx ↔ False := by
+    grind [Rewriter.createEmptyOp, OperationPtr.allocEmpty, Operation.empty, OperationPtr.set, RegionPtr.InBounds]
+  have : ctx.nextID = 1 := by
+    grind [Rewriter.createEmptyOp, OperationPtr.allocEmpty, Operation.empty, OperationPtr.set, RegionPtr.InBounds]
+  have : operation.get ctx (by simp_all) = Operation.empty ModuleTypeID := by
+    grind [Rewriter.createEmptyOp, OperationPtr.allocEmpty, Operation.empty, OperationPtr.set, RegionPtr.InBounds]
+  rlet ctx ← Rewriter.initOpRegions ctx operation 1 (by grind)
+  have : operation = 0 := by grind [Rewriter.createEmptyOp, OperationPtr.allocEmpty]
+  have : ctx.topLevelOp = 0 := by
+    simp_all [Rewriter.initOpRegions, OperationPtr.setRegions, OperationPtr.set, Rewriter.createRegion]
+    grind [RegionPtr.set, RegionPtr.allocEmpty]
+  have hop₀ : ∀ (op : OperationPtr), op.InBounds ctx ↔ op = 0 := by
+    simp_all [Rewriter.initOpRegions, OperationPtr.setRegions, OperationPtr.set, Rewriter.createRegion]
+    simp [OperationPtr.InBounds] at hops
+    grind [Region.empty, RegionPtr.set, OperationPtr.InBounds]
+  have : operation.get ctx (by simp_all) =
+    { Operation.empty ModuleTypeID with regions := #[1] } := by
+    simp_all [Rewriter.initOpRegions, OperationPtr.setRegions, OperationPtr.set, Rewriter.createRegion]
+    grind [Operation.empty, RegionPtr.set, RegionPtr.InBounds, RegionPtr.get, OperationPtr.get, RegionPtr.allocEmpty]
+  have : ∀ (bl : BlockPtr), bl.InBounds ctx ↔ False := by
+    simp_all [Rewriter.initOpRegions, OperationPtr.setRegions, OperationPtr.set, Rewriter.createRegion]
+    grind [Region.empty, RegionPtr.set, BlockPtr.InBounds]
+  have : ∀ (r : RegionPtr), r.InBounds ctx ↔ r = 1 := by
+    simp_all [Rewriter.initOpRegions, OperationPtr.setRegions, OperationPtr.set, Rewriter.createRegion]
+    grind [Region.empty, RegionPtr.set, RegionPtr.InBounds]
+  have : (1 : RegionPtr).get ctx (by simp_all) = Region.empty := by
+    simp_all [Rewriter.initOpRegions, OperationPtr.setRegions, OperationPtr.set, Rewriter.createRegion]
+    grind [Region.empty, RegionPtr.set, RegionPtr.InBounds, RegionPtr.get, RegionPtr.allocEmpty]
+  have : ctx.FieldsInBounds := by
+    constructor
+    · grind [Operation.empty]
+    · sorry -- grind [Operation.FieldsInBounds, Operation.empty]
+    · grind
+    · grind [Region.FieldsInBounds, Region.empty]
+  let moduleRegion := operation.getRegion! ctx 0
+  rlet (ctx, block) ← Rewriter.createBlock ctx (some (BlockInsertPoint.AtEnd moduleRegion)) (by grind) (by sorry)
+  let ctx := { ctx with topLevelOp := operation }
+  (ctx, 0)
