Mlir.lean
@@ -2,7 +2,6 @@ import Mlir.Core.Basic
 import Mlir.Core.Fields
 import Mlir.Core.WellFormed
 import Mlir.Rewriter.LinkedList.WellFormed
-import Mlir.Rewriter.WellFormed.Builder
 import Mlir.Rewriter.WellFormed.Rewriter
 import Mlir.Printer
 import Mlir.PatternRewriter.Basic
