Mlir/Rewriter/WellFormed/Builder/OpOperands.lean
@@ -1,7 +1,7 @@
 import Mlir.Core.Basic
 import Mlir.Core.WellFormed
-import Mlir.Rewriter.Builder
-import Mlir.Rewriter.BuilderInBounds
+import Mlir.Rewriter.Basic
+import Mlir.Rewriter.RewriterGetSetInBounds
 import Mlir.Rewriter.LinkedList.GetSet
 
 namespace Mlir
@@ -12,39 +12,39 @@ variable (opPtr opPtr' : OperationPtr)
 variable (opPtrInBounds : opPtr.InBounds ctx := by grind)
 
 @[simp, grind .]
-theorem Builder.pushOperand_ValuePtr_InBounds_iff (valuePtr : ValuePtr) (hval : valuePtr.InBounds ctx) :
+theorem Rewriter.pushOperand_ValuePtr_InBounds_iff (valuePtr : ValuePtr) (hval : valuePtr.InBounds ctx) :
     ∀ (valuePtr' : ValuePtr), (valuePtr'.InBounds ctx) →
-    (valuePtr'.InBounds (Builder.pushOperand ctx opPtr valuePtr h₁ hval h₃)) := by
-  grind [Builder.pushOperand]
+    (valuePtr'.InBounds (Rewriter.pushOperand ctx opPtr valuePtr h₁ hval h₃)) := by
+  grind [Rewriter.pushOperand]
 
 
 @[simp, grind =]
-theorem Builder.pushOperand_OperandPtr_InBounds_iff (valuePtr : ValuePtr) (hval : valuePtr.InBounds ctx) :
+theorem Rewriter.pushOperand_OperandPtr_InBounds_iff (valuePtr : ValuePtr) (hval : valuePtr.InBounds ctx) :
     ∀ (operandPtr : OpOperandPtr),
-    (operandPtr.InBounds (Builder.pushOperand ctx opPtr valuePtr h₁ hval h₃)) ↔ ((operandPtr.InBounds ctx) ∨ operandPtr = opPtr.nextOperand ctx) := by
-  simp only [Builder.pushOperand]
+    (operandPtr.InBounds (Rewriter.pushOperand ctx opPtr valuePtr h₁ hval h₃)) ↔ ((operandPtr.InBounds ctx) ∨ operandPtr = opPtr.nextOperand ctx) := by
+  simp only [Rewriter.pushOperand]
   simp [←GenericPtr.iff_opOperand]
   grind
 
 @[simp, grind =]
-theorem Builder.pushOperand_ValuePtr_getFirstUse (valuePtr : ValuePtr) (hval : valuePtr.InBounds ctx)
+theorem Rewriter.pushOperand_ValuePtr_getFirstUse (valuePtr : ValuePtr) (hval : valuePtr.InBounds ctx)
     (valuePtr' : ValuePtr) (valuePtrInBounds' : valuePtr'.InBounds ctx) :
-    valuePtr'.getFirstUse (Builder.pushOperand ctx opPtr valuePtr h₁ hval h₂) (by grind) =
+    valuePtr'.getFirstUse (Rewriter.pushOperand ctx opPtr valuePtr h₁ hval h₂) (by grind) =
     if valuePtr = valuePtr' then
       some (opPtr.nextOperand ctx)
     else
       valuePtr'.getFirstUse ctx := by
   sorry -- TODO
-  -- grind [Builder.pushOperand]
+  -- grind [Rewriter.pushOperand]
 
-theorem Builder.pushOperand_OpOperandPtr_get_firstUse (valuePtr : ValuePtr)
+theorem Rewriter.pushOperand_OpOperandPtr_get_firstUse (valuePtr : ValuePtr)
     valuePtrInBounds (oldFirstUse : OpOperandPtr) (hold : oldFirstUse.InBounds ctx)
     (hOldFirstUse : valuePtr.getFirstUse ctx valuePtrInBounds = some oldFirstUse) :
-      oldFirstUse.get (Builder.pushOperand ctx opPtr valuePtr opPtrInBounds valuePtrInBounds ctxInBounds) =
+      oldFirstUse.get (Rewriter.pushOperand ctx opPtr valuePtr opPtrInBounds valuePtrInBounds ctxInBounds) =
           {oldFirstUse.get ctx (by grind) with back := OpOperandPtrPtr.operandNextUse (opPtr.nextOperand ctx)}
       := by
   simp only [←OpOperandPtr.get!_eq_get]
-  simp only [Builder.pushOperand]
+  simp only [Rewriter.pushOperand]
   sorry
   -- rw [OpOperandPtr.get!_insertIntoCurrent _ (by grind [OpOperand.FieldsInBounds]) (by grind)]
   -- · split
@@ -57,23 +57,23 @@ theorem Builder.pushOperand_OpOperandPtr_get_firstUse (valuePtr : ValuePtr)
   -- · grind [OpOperandPtr.InBounds, OperationPtr.get]
 
 include ctxInBounds in
-theorem Builder.pushOperand_OpOperandPtr_get_newOperand (valuePtr : ValuePtr) valuePtrInBounds :
-    (opPtr.nextOperand ctx).get (Builder.pushOperand ctx opPtr valuePtr opPtrInBounds valuePtrInBounds ctxInBounds) (by grind) =
+theorem Rewriter.pushOperand_OpOperandPtr_get_newOperand (valuePtr : ValuePtr) valuePtrInBounds :
+    (opPtr.nextOperand ctx).get (Rewriter.pushOperand ctx opPtr valuePtr opPtrInBounds valuePtrInBounds ctxInBounds) (by grind) =
       { value := valuePtr,
         owner := opPtr,
         back := .valueFirstUse valuePtr,
         nextUse := (valuePtr.getFirstUse ctx valuePtrInBounds) } := by
-  simp [Builder.pushOperand, ←OpOperandPtr.get!_eq_get]
+  simp [Rewriter.pushOperand, ←OpOperandPtr.get!_eq_get]
   grind
 
-theorem Builder.pushOperand_OpOperandPtr_other (valuePtr : ValuePtr) (valuePtrInBounds : valuePtr.InBounds ctx) :
+theorem Rewriter.pushOperand_OpOperandPtr_other (valuePtr : ValuePtr) (valuePtrInBounds : valuePtr.InBounds ctx) :
     ∀ (operandPtr : OpOperandPtr) (operandPtrInBounds : operandPtr.InBounds ctx)
       (_operandPtrNeFirstUse : valuePtr.getFirstUse ctx valuePtrInBounds ≠ some operandPtr),
-      operandPtr.get (Builder.pushOperand ctx opPtr valuePtr opPtrInBounds valuePtrInBounds ctxInBounds) (by grind) =
+      operandPtr.get (Rewriter.pushOperand ctx opPtr valuePtr opPtrInBounds valuePtrInBounds ctxInBounds) (by grind) =
         operandPtr.get ctx := by
   intros operandPtr operandPtrInBounds operandPtrNeFirstUse
   simp only [←OpOperandPtr.get!_eq_get]
-  simp only [Builder.pushOperand, OpOperandPtr.insertIntoCurrent]
+  simp only [Rewriter.pushOperand, OpOperandPtr.insertIntoCurrent]
   -- simp only [OpOperandPtr.get_OperationPtr_setOperands, ↓reduceDIte, Array.getElem_push_eq,
   --   ValuePtr.getFirstUse_OpOperandPtr_setBack, ValuePtr.getFirstUse_OperationPtr_setOperands]
   -- split <;> simp_all <;> grind [OpOperandPtr.InBounds, OperationPtr.get, OpOperandPtr.get]
@@ -81,10 +81,10 @@ theorem Builder.pushOperand_OpOperandPtr_other (valuePtr : ValuePtr) (valuePtrIn
 
 include ctxInBounds in
 @[grind =]
-theorem Builder.pushOperand_OpOperandPtr_get
+theorem Rewriter.pushOperand_OpOperandPtr_get
     (valuePtr : ValuePtr) valuePtrInBounds (operandPtr : OpOperandPtr)
-    (operandPtrInBounds : operandPtr.InBounds (Builder.pushOperand ctx opPtr valuePtr opPtrInBounds valuePtrInBounds ctxInBounds)) :
-    operandPtr.get (Builder.pushOperand ctx opPtr valuePtr opPtrInBounds valuePtrInBounds ctxInBounds) operandPtrInBounds =
+    (operandPtrInBounds : operandPtr.InBounds (Rewriter.pushOperand ctx opPtr valuePtr opPtrInBounds valuePtrInBounds ctxInBounds)) :
+    operandPtr.get (Rewriter.pushOperand ctx opPtr valuePtr opPtrInBounds valuePtrInBounds ctxInBounds) operandPtrInBounds =
       if h : operandPtr = opPtr.nextOperand ctx then
         { value := valuePtr,
           owner := opPtr,
@@ -94,19 +94,19 @@ theorem Builder.pushOperand_OpOperandPtr_get
        { operandPtr.get ctx (by grind) with back := OpOperandPtrPtr.operandNextUse (opPtr.nextOperand ctx) }
       else
         operandPtr.get ctx (by grind) := by
-  grind [Builder.pushOperand_OpOperandPtr_other, Builder.pushOperand_OpOperandPtr_get_newOperand, Builder.pushOperand_OpOperandPtr_get_firstUse]
+  grind [Rewriter.pushOperand_OpOperandPtr_other, Rewriter.pushOperand_OpOperandPtr_get_newOperand, Rewriter.pushOperand_OpOperandPtr_get_firstUse]
 
 include ctxInBounds in
 @[simp, grind.]
-theorem Builder.pushOperand_WellFormedUseDefChain_getElem?
+theorem Rewriter.pushOperand_WellFormedUseDefChain_getElem?
     (valuePtr : ValuePtr) (valuePtrInBounds : valuePtr.InBounds ctx)
     array (arrayWf : valuePtr.WellFormedUseDefChain ctx array) (i : Nat) (hISize : i < array.size) :
-    (array[i].get (Builder.pushOperand ctx opPtr valuePtr opPtrInBounds valuePtrInBounds ctxInBounds) (by grind [ValuePtr.WellFormedUseDefChain])) =
+    (array[i].get (Rewriter.pushOperand ctx opPtr valuePtr opPtrInBounds valuePtrInBounds ctxInBounds) (by grind [ValuePtr.WellFormedUseDefChain])) =
       { (OpOperandPtr.get array[i] ctx (by grind [ValuePtr.WellFormedUseDefChain])) with
         back := (if i = 0 then .operandNextUse (opPtr.nextOperand ctx) else (OpOperandPtr.get array[i] ctx (by grind [ValuePtr.WellFormedUseDefChain])).back) }
     := by
   simp only
-  simp (disch := grind) only [Builder.pushOperand_OpOperandPtr_get]
+  simp (disch := grind) only [Rewriter.pushOperand_OpOperandPtr_get]
   split
   · grind
   · split
@@ -115,10 +115,10 @@ theorem Builder.pushOperand_WellFormedUseDefChain_getElem?
       simp [this]
 
 set_option maxHeartbeats 10000000 in -- TODO
-theorem Builder.pushOperand_WellFormedUseDefChain
+theorem Rewriter.pushOperand_WellFormedUseDefChain
     (valuePtr : ValuePtr) (valuePtrInBounds : valuePtr.InBounds ctx) (hOpWf : ctx.WellFormed)
     (valuePtr' : ValuePtr) (valuePtr'InBounds : valuePtr'.InBounds ctx) :
-    ∃ array, valuePtr'.WellFormedUseDefChain (Builder.pushOperand ctx opPtr valuePtr opPtrInBounds valuePtrInBounds ctxInBounds) array (by grind) := by
+    ∃ array, valuePtr'.WellFormedUseDefChain (Rewriter.pushOperand ctx opPtr valuePtr opPtrInBounds valuePtrInBounds ctxInBounds) array (by grind) := by
   have ⟨array', arrayWf'⟩ := hOpWf.valueUseDefChains valuePtr' valuePtr'InBounds
   have ⟨array, arrayWf⟩ := hOpWf.valueUseDefChains valuePtr valuePtrInBounds
   by_cases valuePtr' = valuePtr
@@ -153,169 +153,169 @@ theorem Builder.pushOperand_WellFormedUseDefChain
       grind [ValuePtr.WellFormedUseDefChain]
 
 -- /--
--- info: 'Mlir.Builder.pushOperand_WellFormedUseDefChain' depends on axioms: [propext, Classical.choice, Quot.sound]
+-- info: 'Mlir.Rewriter.pushOperand_WellFormedUseDefChain' depends on axioms: [propext, Classical.choice, Quot.sound]
 -- -/
 -- #guard_msgs in
--- #print axioms Builder.pushOperand_WellFormedUseDefChain
+-- #print axioms Rewriter.pushOperand_WellFormedUseDefChain
 
-theorem Builder.pushOperand_BlockOperand_get (valuePtr : ValuePtr) (valuePtrInBounds : valuePtr.InBounds ctx) :
+theorem Rewriter.pushOperand_BlockOperand_get (valuePtr : ValuePtr) (valuePtrInBounds : valuePtr.InBounds ctx) :
     ∀ (blockOperandPtr : BlockOperandPtr) (hInBounds : blockOperandPtr.InBounds ctx) blockInBounds,
-      blockOperandPtr.get (Builder.pushOperand ctx opPtr valuePtr opPtrInBounds valuePtrInBounds ctxInBounds) blockInBounds = blockOperandPtr.get ctx hInBounds := by
-  simp only [Builder.pushOperand]
+      blockOperandPtr.get (Rewriter.pushOperand ctx opPtr valuePtr opPtrInBounds valuePtrInBounds ctxInBounds) blockInBounds = blockOperandPtr.get ctx hInBounds := by
+  simp only [Rewriter.pushOperand]
   grind
 
-theorem Builder.pushOperand_BlockPtr_get_firstUse_mono (valuePtr : ValuePtr) (valuePtrInBounds : valuePtr.InBounds ctx) :
+theorem Rewriter.pushOperand_BlockPtr_get_firstUse_mono (valuePtr : ValuePtr) (valuePtrInBounds : valuePtr.InBounds ctx) :
     ∀ (blockPtr : BlockPtr) hBlockInBounds,
-      (blockPtr.get (Builder.pushOperand ctx opPtr valuePtr opPtrInBounds valuePtrInBounds ctxInBounds) hBlockInBounds).firstUse =
+      (blockPtr.get (Rewriter.pushOperand ctx opPtr valuePtr opPtrInBounds valuePtrInBounds ctxInBounds) hBlockInBounds).firstUse =
         (blockPtr.get ctx (by grind)).firstUse := by
-  grind [Builder.pushOperand]
+  grind [Rewriter.pushOperand]
 
-theorem Builder.pushOperand_BlockPtr_get_firstOp_mono (valuePtr : ValuePtr) (valuePtrInBounds : valuePtr.InBounds ctx) :
+theorem Rewriter.pushOperand_BlockPtr_get_firstOp_mono (valuePtr : ValuePtr) (valuePtrInBounds : valuePtr.InBounds ctx) :
     ∀ (blockPtr : BlockPtr) hBlockInBounds,
-      (blockPtr.get (Builder.pushOperand ctx opPtr valuePtr opPtrInBounds valuePtrInBounds ctxInBounds) hBlockInBounds).firstOp =
+      (blockPtr.get (Rewriter.pushOperand ctx opPtr valuePtr opPtrInBounds valuePtrInBounds ctxInBounds) hBlockInBounds).firstOp =
         (blockPtr.get ctx (by grind)).firstOp := by
-  grind [Builder.pushOperand]
+  grind [Rewriter.pushOperand]
 
-theorem Builder.pushOperand_BlockPtr_get_lastOp_mono (valuePtr : ValuePtr) (valuePtrInBounds : valuePtr.InBounds ctx) :
+theorem Rewriter.pushOperand_BlockPtr_get_lastOp_mono (valuePtr : ValuePtr) (valuePtrInBounds : valuePtr.InBounds ctx) :
     ∀ (blockPtr : BlockPtr) hBlockInBounds,
-      (blockPtr.get (Builder.pushOperand ctx opPtr valuePtr opPtrInBounds valuePtrInBounds ctxInBounds) hBlockInBounds).lastOp =
+      (blockPtr.get (Rewriter.pushOperand ctx opPtr valuePtr opPtrInBounds valuePtrInBounds ctxInBounds) hBlockInBounds).lastOp =
         (blockPtr.get ctx (by grind)).lastOp := by
-  grind [Builder.pushOperand]
+  grind [Rewriter.pushOperand]
 
 
-theorem Builder.pushOperand_OperationPtr_get_parent_mono (valuePtr : ValuePtr) (valuePtrInBounds : valuePtr.InBounds ctx) hOp'InBounds :
-      (opPtr'.get (Builder.pushOperand ctx opPtr valuePtr opPtrInBounds valuePtrInBounds ctxInBounds) hOp'InBounds).parent =
+theorem Rewriter.pushOperand_OperationPtr_get_parent_mono (valuePtr : ValuePtr) (valuePtrInBounds : valuePtr.InBounds ctx) hOp'InBounds :
+      (opPtr'.get (Rewriter.pushOperand ctx opPtr valuePtr opPtrInBounds valuePtrInBounds ctxInBounds) hOp'InBounds).parent =
         (opPtr'.get ctx (by grind)).parent := by
-  grind [Builder.pushOperand]
+  grind [Rewriter.pushOperand]
 
 @[grind =]
-theorem Builder.BlockPtr_get_pushOperand_parent (bl : BlockPtr) (hin : bl.InBounds ctx) :
-    (bl.get (Builder.pushOperand ctx opPtr valuePtr opPtrInBounds valuePtrInBounds ctxInBounds)).parent =
+theorem Rewriter.BlockPtr_get_pushOperand_parent (bl : BlockPtr) (hin : bl.InBounds ctx) :
+    (bl.get (Rewriter.pushOperand ctx opPtr valuePtr opPtrInBounds valuePtrInBounds ctxInBounds)).parent =
     (bl.get ctx hin).parent := by
-  grind [Builder.pushOperand]
+  grind [Rewriter.pushOperand]
 
 @[grind =]
-theorem Builder.BlockPtr_get_pushOperand_prev (bl : BlockPtr) (hin : bl.InBounds ctx) :
-    (bl.get (Builder.pushOperand ctx opPtr valuePtr opPtrInBounds valuePtrInBounds ctxInBounds)).prev =
+theorem Rewriter.BlockPtr_get_pushOperand_prev (bl : BlockPtr) (hin : bl.InBounds ctx) :
+    (bl.get (Rewriter.pushOperand ctx opPtr valuePtr opPtrInBounds valuePtrInBounds ctxInBounds)).prev =
     (bl.get ctx hin).prev := by
-  grind [Builder.pushOperand]
+  grind [Rewriter.pushOperand]
 
 @[grind =]
-theorem Builder.BlockPtr_get_pushOperand_next (bl : BlockPtr) (hin : bl.InBounds ctx) :
-    (bl.get (Builder.pushOperand ctx opPtr valuePtr opPtrInBounds valuePtrInBounds ctxInBounds)).next =
+theorem Rewriter.BlockPtr_get_pushOperand_next (bl : BlockPtr) (hin : bl.InBounds ctx) :
+    (bl.get (Rewriter.pushOperand ctx opPtr valuePtr opPtrInBounds valuePtrInBounds ctxInBounds)).next =
     (bl.get ctx hin).next := by
-  grind [Builder.pushOperand]
+  grind [Rewriter.pushOperand]
 
 @[simp, grind =]
-theorem BlockPtr.getNumArguments!_Builder_pushOperand :
-    BlockPtr.getNumArguments! block (Builder.pushOperand ctx opPtr valuePtr opPtrInBounds valuePtrInBounds ctxInBounds) =
+theorem BlockPtr.getNumArguments!_Rewriter_pushOperand :
+    BlockPtr.getNumArguments! block (Rewriter.pushOperand ctx opPtr valuePtr opPtrInBounds valuePtrInBounds ctxInBounds) =
     BlockPtr.getNumArguments! block ctx := by
-  grind [Builder.pushOperand]
+  grind [Rewriter.pushOperand]
 
 @[simp, grind =]
-theorem BlockArgumentPtr.index!_Builder_pushOperand :
-    (BlockArgumentPtr.get! arg (Builder.pushOperand ctx opPtr valuePtr opPtrInBounds valuePtrInBounds ctxInBounds)).index =
+theorem BlockArgumentPtr.index!_Rewriter_pushOperand :
+    (BlockArgumentPtr.get! arg (Rewriter.pushOperand ctx opPtr valuePtr opPtrInBounds valuePtrInBounds ctxInBounds)).index =
     (BlockArgumentPtr.get! arg ctx).index := by
-  grind [Builder.pushOperand]
+  grind [Rewriter.pushOperand]
 
 @[simp, grind =]
-theorem BlockArgumentPtr.owner!_Builder_pushOperand :
-    (BlockArgumentPtr.get! arg (Builder.pushOperand ctx opPtr valuePtr opPtrInBounds valuePtrInBounds ctxInBounds)).owner =
+theorem BlockArgumentPtr.owner!_Rewriter_pushOperand :
+    (BlockArgumentPtr.get! arg (Rewriter.pushOperand ctx opPtr valuePtr opPtrInBounds valuePtrInBounds ctxInBounds)).owner =
     (BlockArgumentPtr.get! arg ctx).owner := by
-  grind [Builder.pushOperand]
+  grind [Rewriter.pushOperand]
 
 @[grind =]
-theorem Builder.RegionPtr_get_pushOperand (rg : RegionPtr) (hin : rg.InBounds ctx) :
-    rg.get (Builder.pushOperand ctx opPtr valuePtr opPtrInBounds valuePtrInBounds ctxInBounds) =
+theorem Rewriter.RegionPtr_get_pushOperand (rg : RegionPtr) (hin : rg.InBounds ctx) :
+    rg.get (Rewriter.pushOperand ctx opPtr valuePtr opPtrInBounds valuePtrInBounds ctxInBounds) =
     rg.get ctx hin := by
-  grind [Builder.pushOperand]
+  grind [Rewriter.pushOperand]
 
-theorem Builder.pushOperand_OperationPtr_get_next_mono (valuePtr : ValuePtr) (valuePtrInBounds : valuePtr.InBounds ctx) hOp'InBounds :
-      (opPtr'.get (Builder.pushOperand ctx opPtr valuePtr opPtrInBounds valuePtrInBounds ctxInBounds) hOp'InBounds).next =
+theorem Rewriter.pushOperand_OperationPtr_get_next_mono (valuePtr : ValuePtr) (valuePtrInBounds : valuePtr.InBounds ctx) hOp'InBounds :
+      (opPtr'.get (Rewriter.pushOperand ctx opPtr valuePtr opPtrInBounds valuePtrInBounds ctxInBounds) hOp'InBounds).next =
         (opPtr'.get ctx (by grind)).next := by
-  grind [Builder.pushOperand]
+  grind [Rewriter.pushOperand]
 
-theorem Builder.pushOperand_OperationPtr_get_prev_mono (valuePtr : ValuePtr) (valuePtrInBounds : valuePtr.InBounds ctx) hOp'InBounds :
-      (opPtr'.get (Builder.pushOperand ctx opPtr valuePtr opPtrInBounds valuePtrInBounds ctxInBounds) hOp'InBounds).prev =
+theorem Rewriter.pushOperand_OperationPtr_get_prev_mono (valuePtr : ValuePtr) (valuePtrInBounds : valuePtr.InBounds ctx) hOp'InBounds :
+      (opPtr'.get (Rewriter.pushOperand ctx opPtr valuePtr opPtrInBounds valuePtrInBounds ctxInBounds) hOp'InBounds).prev =
         (opPtr'.get ctx (by grind)).prev := by
-  grind [Builder.pushOperand]
+  grind [Rewriter.pushOperand]
 
 @[simp, grind =]
-theorem Builder.pushOperand_OperationPtr_getNumRegions (valuePtr : ValuePtr) (valuePtrInBounds : valuePtr.InBounds ctx) hOp'InBounds :
-      opPtr'.getNumRegions (Builder.pushOperand ctx opPtr valuePtr opPtrInBounds valuePtrInBounds ctxInBounds) hOp'InBounds =
+theorem Rewriter.pushOperand_OperationPtr_getNumRegions (valuePtr : ValuePtr) (valuePtrInBounds : valuePtr.InBounds ctx) hOp'InBounds :
+      opPtr'.getNumRegions (Rewriter.pushOperand ctx opPtr valuePtr opPtrInBounds valuePtrInBounds ctxInBounds) hOp'InBounds =
         opPtr'.getNumRegions ctx (by grind) := by
-  simp only [Builder.pushOperand, OpOperandPtr.insertIntoCurrent]
+  simp only [Rewriter.pushOperand, OpOperandPtr.insertIntoCurrent]
   grind
 
 @[simp, grind =]
-theorem Builder.pushOperand_OperationPtr_getRegion (valuePtr : ValuePtr) (valuePtrInBounds : valuePtr.InBounds ctx) :
-      opPtr'.getRegion! (Builder.pushOperand ctx opPtr valuePtr opPtrInBounds valuePtrInBounds ctxInBounds) =
+theorem Rewriter.pushOperand_OperationPtr_getRegion (valuePtr : ValuePtr) (valuePtrInBounds : valuePtr.InBounds ctx) :
+      opPtr'.getRegion! (Rewriter.pushOperand ctx opPtr valuePtr opPtrInBounds valuePtrInBounds ctxInBounds) =
         opPtr'.getRegion! ctx := by
-  simp only [Builder.pushOperand, OpOperandPtr.insertIntoCurrent]
+  simp only [Rewriter.pushOperand, OpOperandPtr.insertIntoCurrent]
   grind
 
 @[grind =]
-theorem Builder.pushOperand_RegionPtr_get (rgPtr : RegionPtr) hRgInBounds :
-      (rgPtr.get (Builder.pushOperand ctx opPtr valuePtr opPtrInBounds valuePtrInBounds ctxInBounds) hRgInBounds) =
+theorem Rewriter.pushOperand_RegionPtr_get (rgPtr : RegionPtr) hRgInBounds :
+      (rgPtr.get (Rewriter.pushOperand ctx opPtr valuePtr opPtrInBounds valuePtrInBounds ctxInBounds) hRgInBounds) =
         (rgPtr.get ctx (by grind)) := by
-  grind [Builder.pushOperand]
+  grind [Rewriter.pushOperand]
 
 @[grind =]
-theorem Builder.pushOperand_OperationPtr_get_num_results (valuePtr : ValuePtr) (valuePtrInBounds : valuePtr.InBounds ctx) :
-      opPtr'.getNumResults! (Builder.pushOperand ctx opPtr valuePtr opPtrInBounds valuePtrInBounds ctxInBounds) =
+theorem Rewriter.pushOperand_OperationPtr_get_num_results (valuePtr : ValuePtr) (valuePtrInBounds : valuePtr.InBounds ctx) :
+      opPtr'.getNumResults! (Rewriter.pushOperand ctx opPtr valuePtr opPtrInBounds valuePtrInBounds ctxInBounds) =
       opPtr'.getNumResults! ctx := by
-  grind [Builder.pushOperand]
+  grind [Rewriter.pushOperand]
 
 @[simp, grind =]
-theorem OperationPtr.getNumSuccessors!_Builder_pushOperand (valuePtr : ValuePtr) (valuePtrInBounds : valuePtr.InBounds ctx) :
-    opPtr'.getNumSuccessors! (Builder.pushOperand ctx opPtr valuePtr opPtrInBounds valuePtrInBounds ctxInBounds) =
+theorem OperationPtr.getNumSuccessors!_Rewriter_pushOperand (valuePtr : ValuePtr) (valuePtrInBounds : valuePtr.InBounds ctx) :
+    opPtr'.getNumSuccessors! (Rewriter.pushOperand ctx opPtr valuePtr opPtrInBounds valuePtrInBounds ctxInBounds) =
     opPtr'.getNumSuccessors! ctx := by
-  grind [Builder.pushOperand]
+  grind [Rewriter.pushOperand]
 
 @[simp, grind =]
-theorem BlockOperandPtr.get!_Builder_pushOperand (valuePtr : ValuePtr) (valuePtrInBounds : valuePtr.InBounds ctx)
+theorem BlockOperandPtr.get!_Rewriter_pushOperand (valuePtr : ValuePtr) (valuePtrInBounds : valuePtr.InBounds ctx)
     (blockOperandPtr : BlockOperandPtr) :
-    blockOperandPtr.get! (Builder.pushOperand ctx opPtr valuePtr opPtrInBounds valuePtrInBounds ctxInBounds) =
+    blockOperandPtr.get! (Rewriter.pushOperand ctx opPtr valuePtr opPtrInBounds valuePtrInBounds ctxInBounds) =
     blockOperandPtr.get! ctx := by
-  grind [Builder.pushOperand]
+  grind [Rewriter.pushOperand]
 
 @[simp, grind =]
 theorem OpResultPtr.index_pushOperand :
-    (OpResultPtr.get result (Builder.pushOperand ctx opPtr valuePtr opPtrInBounds valuePtrInBounds ctxInBounds) h).index =
+    (OpResultPtr.get result (Rewriter.pushOperand ctx opPtr valuePtr opPtrInBounds valuePtrInBounds ctxInBounds) h).index =
     (OpResultPtr.get result ctx (by grind)).index := by
-  grind [Builder.pushOperand]
+  grind [Rewriter.pushOperand]
 
 @[simp, grind =]
 theorem OpOperandPtr.OperationPtr_get_pushOperand_operands_size (op : OperationPtr)
     (h : op.InBounds ctx) opPtrInBounds :
-    op.getNumOperands (Builder.pushOperand ctx opPtr valuePtr opPtrInBounds valuePtrInBounds ctxInBounds) =
+    op.getNumOperands (Rewriter.pushOperand ctx opPtr valuePtr opPtrInBounds valuePtrInBounds ctxInBounds) =
     if op = opPtr then op.getNumOperands ctx + 1 else op.getNumOperands ctx := by
-  simp only [Builder.pushOperand]
+  simp only [Rewriter.pushOperand]
   grind
 
 @[grind =]
 theorem OpOperandPtr.OperationPtr_get_pushOperand_operands_owner {opr : OpOperandPtr} {h} :
-    (opr.get (Builder.pushOperand ctx opPtr valuePtr opPtrInBounds valuePtrInBounds ctxInBounds) h).owner =
+    (opr.get (Rewriter.pushOperand ctx opPtr valuePtr opPtrInBounds valuePtrInBounds ctxInBounds) h).owner =
     if h: opr = opPtr.nextOperand ctx then
       opPtr
     else
       (opr.get ctx).owner := by
-  grind [Builder.pushOperand]
+  grind [Rewriter.pushOperand]
 
-theorem Builder.pushOperand_WellFormed  (valuePtr : ValuePtr) (valuePtrInBounds : valuePtr.InBounds ctx) (hOpWf : ctx.WellFormed) :
-    (Builder.pushOperand ctx opPtr valuePtr opPtrInBounds valuePtrInBounds ctxInBounds).WellFormed := by
+theorem Rewriter.pushOperand_WellFormed  (valuePtr : ValuePtr) (valuePtrInBounds : valuePtr.InBounds ctx) (hOpWf : ctx.WellFormed) :
+    (Rewriter.pushOperand ctx opPtr valuePtr opPtrInBounds valuePtrInBounds ctxInBounds).WellFormed := by
   constructor
   case valueUseDefChains =>
-    grind [Builder.pushOperand_WellFormedUseDefChain]
+    grind [Rewriter.pushOperand_WellFormedUseDefChain]
   case blockUseDefChains =>
     intros blockPtr blockPtrInBounds
     have ⟨array, arrayWf⟩ := hOpWf.blockUseDefChains blockPtr (by grind)
     exists array
     apply IRContext.BlockPtr_UseDefChainWellFormed_unchanged (ctx := ctx)
     · grind [IRContext.WellFormed]
-    · grind [Builder.pushOperand_BlockOperand_get]
-    · grind [Builder.pushOperand_BlockPtr_get_firstUse_mono]
-    · grind [Builder.pushOperand_BlockOperand_get]
+    · grind [Rewriter.pushOperand_BlockOperand_get]
+    · grind [Rewriter.pushOperand_BlockPtr_get_firstUse_mono]
+    · grind [Rewriter.pushOperand_BlockOperand_get]
     · grind
     · grind
   case inBounds => grind
@@ -341,7 +341,7 @@ theorem Builder.pushOperand_WellFormed  (valuePtr : ValuePtr) (valuePtrInBounds 
       intros region regionInBounds
       simp only [pushOperand_OperationPtr_getRegion]
       grind
-    all_goals grind [Builder.pushOperand, Operation.WellFormed, OperationPtr.getOpOperand]
+    all_goals grind [Rewriter.pushOperand, Operation.WellFormed, OperationPtr.getOpOperand]
   case blocks =>
     intros bl hbl
     constructor
@@ -356,23 +356,23 @@ theorem Builder.pushOperand_WellFormed  (valuePtr : ValuePtr) (valuePtrInBounds 
     intros reg hreg
     have ⟨h₁, h₂⟩ := hOpWf.regions reg (by grind)
     constructor
-    · grind [Builder.pushOperand]
+    · grind [Rewriter.pushOperand]
     · grind
 
 -- /--
--- info: 'Mlir.Builder.pushOperand_WellFormed' depends on axioms: [propext, Classical.choice, Quot.sound]
+-- info: 'Mlir.Rewriter.pushOperand_WellFormed' depends on axioms: [propext, Classical.choice, Quot.sound]
 -- -/
 -- #guard_msgs in
--- #print axioms Builder.pushOperand_WellFormed
+-- #print axioms Rewriter.pushOperand_WellFormed
 
-theorem Builder.initOpOperands_WellFormed (ctx: IRContext) (opPtr: OperationPtr) (opPtrInBounds : opPtr.InBounds ctx)
+theorem Rewriter.initOpOperands_WellFormed (ctx: IRContext) (opPtr: OperationPtr) (opPtrInBounds : opPtr.InBounds ctx)
     (operands : Array ValuePtr) (hoperands : ∀ oper, oper ∈ operands → oper.InBounds ctx) (hctx : ctx.FieldsInBounds)
     (n : Nat := operands.size) (hn : 0 ≤ n ∧ n ≤ operands.size := by grind)
     (hOpWf : ctx.WellFormed) :
-    (Builder.initOpOperands ctx opPtr opPtrInBounds operands hoperands hctx n hn).WellFormed := by
+    (Rewriter.initOpOperands ctx opPtr opPtrInBounds operands hoperands hctx n hn).WellFormed := by
   induction n generalizing ctx
   case zero =>
     grind [initOpOperands]
   case succ n ih =>
     simp only [initOpOperands]
-    grind [Builder.pushOperand_WellFormed]
+    grind [Rewriter.pushOperand_WellFormed]
