Mlir/Rewriter/WellFormed/Builder/OpRegion.lean
@@ -1,11 +1,11 @@
 import Mlir.Core.Basic
 import Mlir.Core.WellFormed
-import Mlir.Rewriter.Builder
+import Mlir.Rewriter.Basic
 
 namespace Mlir
 
-theorem Builder.initOpRegions_WellFormed (ctx: IRContext) (opPtr: OperationPtr) (numRegions: Nat)
+theorem Rewriter.initOpRegions_WellFormed (ctx: IRContext) (opPtr: OperationPtr) (numRegions: Nat)
     (hop : opPtr.InBounds ctx) (hctx : IRContext.WellFormed ctx) (newCtx : IRContext):
-    Builder.initOpRegions ctx opPtr numRegions hop = some newCtx →
+    Rewriter.initOpRegions ctx opPtr numRegions hop = some newCtx →
     newCtx.WellFormed := by
   sorry
